ComputationBook/Chapters/MathlibCopy.lean
@@ -1,0 +1,277 @@
+import Mathlib.Data.Countable.Small
+import Mathlib.Data.Fintype.Pigeonhole
+import Mathlib.Tactic.NormNum
+-- import Mathlib.Computability.Language
+/-
+The following is an attempt to understand Mathlibs implementation of DFAs and
+NFAs. I will copy down their code and explain anything I don't understand along
+the way.
+-/
+
+universe u v
+
+
+structure DFA (Q : Type u) (σ : Type v) where
+  δ : Q → σ → Q
+  q₀ : Q
+  F : Set Q
+
+variable {Q : Type u} {σ : Type v}
+
+namespace DFA
+
+/- TODO: Make DFA inductive, and give it a product constructor so that Prod M1 M2 is a DFA-/
+
+/-- `M.evalFrom s x` evaluates `M` with input `x` starting from the state `s`. -/
+
+
+@[simp]
+def evalFrom (M : DFA Q σ) (s : Q) : List σ → Q :=
+  List.foldl M.δ s
+
+/-Running on empty string doesn't change state.-/
+theorem evalFrom_nil (M : DFA Q σ) (s : Q) : evalFrom M s [] = s :=
+  rfl
+
+/-Running DFA on string of length 1 is the same as applying step once.-/
+@[simp]
+theorem evalFrom_singleton (M : DFA Q σ) (s : Q) (a : σ) : evalFrom M s [a] = M.δ s a :=
+  rfl
+
+/-Running a DFA on a string x with `a` appended gives the same state as
+running on the string x and then stepping from that state using `a`. -/
+@[simp]
+theorem evalFrom_append_singleton (M : DFA Q σ) (s : Q) (x : List σ) (a : σ) :
+  evalFrom M s (x ++ [a]) = M.δ (evalFrom M s x) a := by
+    simp[evalFrom]
+
+/-- `M.eval x` evaluates `M` with input `x` starting from the state `M.start`. -/
+@[simp]
+def eval (M : DFA Q σ): List σ → Q :=
+  evalFrom M M.q₀
+
+@[simp]
+theorem eval_nil (M : DFA Q σ) : eval M [] = M.q₀ :=
+  rfl
+
+@[simp]
+theorem eval_singleton (M : DFA Q σ) (a : σ) : eval M [a] = M.δ M.q₀ a :=
+ rfl
+
+@[simp]
+theorem eval_append_singleton (M : DFA Q σ) (x : List σ) (a : σ) :
+eval M (x ++ [a]) = M.δ (eval M x) a :=
+  evalFrom_append_singleton _ _ _ _
+
+theorem evalFrom_of_append (M : DFA Q σ) (start : Q) (x y : List σ) :
+  evalFrom M start (x ++ y) = evalFrom M (evalFrom M start x) y :=
+  List.foldl_append
+
+
+@[simp]
+def acceptsFrom (M : DFA Q σ) (s : Q) : Set (List σ) := {x | evalFrom M s x ∈ M.F}
+
+@[simp]
+def L (M : DFA Q σ) : Set (List σ) := acceptsFrom M M.q₀
+
+/- Proof that the textbook definitions and the lean definitions imply each other. -/
+@[simp]
+def accepts' (M : DFA Q σ) (x : List σ) :=
+  ∃ r : Fin (x.length + 1) → Q,
+  (r 0 = M.q₀) ∧
+  (∀ i : Fin (x.length), M.δ (r (i.castSucc)) x[i] = r (i.castSucc + 1)) ∧
+  (r ⟨ x.length, by simp ⟩ ∈ M.F)
+
+def L' (M : DFA Q σ) : Set (List σ) := {x | accepts' M x}
+
+theorem lang_def_eq (M : DFA Q σ) (x : List σ) : x ∈ L M ↔ x ∈ L' M := by
+  unfold L L' acceptsFrom accepts' evalFrom
+  apply Iff.intro
+  · intro hx
+    exists fun i => List.foldl M.δ M.q₀ (x.take i.val)
+    constructor
+    · simp
+    · constructor
+      · intro i
+        simp
+        have : List.take (↑i + 1) x = List.take (↑i) x ++ [x[↑i]] := by simp
+        rw[this,List.foldl_concat]
+        rfl
+      · simp
+        exact hx
+  · intro ⟨r, h_init, h_trans, h_accept⟩
+    simp
+    have : ∀ i : Fin (x.length + 1), r i = List.foldl M.δ M.q₀ (x.take i) := by
+      intro i
+      induction i using Fin.induction with
+      | zero => simp; exact h_init
+      | succ i ih =>
+      simp at h_trans
+      rw[←h_trans i]
+      have : List.take (i.succ) x = List.take (↑i) x ++ [x[↑i]] := by simp
+      rw[this,List.foldl_concat,ih]
+      rfl
+    have final_eq := this ⟨x.length, by simp⟩
+    rw[final_eq] at h_accept; simp at h_accept
+    exact h_accept
+
+
+
+
+
+
+
+
+
+
+
+variable {Q₁ : Type u}
+universe w
+variable {Q₂ : Type w} (M₁ : DFA Q₁ σ) (M₂ : DFA Q₂ σ)
+
+@[simp]
+def product_of_automata (M₁ : DFA Q₁ σ) (M₂ : DFA Q₂ σ) :
+DFA (Q₁ × Q₂) σ :=
+⟨
+  fun (q₁, q₂) s => (M₁.δ q₁ s, M₂.δ q₂ s),
+  (M₁.q₀, M₂.q₀),
+  { (q₁, q₂) | (q₁ ∈ M₁.F) ∨ (q₂ ∈ M₂.F) }
+⟩
+
+
+@[simp]
+theorem foldl_prod_eq (M₁ : DFA Q₁ σ) (M₂ : DFA Q₂ σ) (x : List σ) :
+  List.foldl (product_of_automata M₁ M₂).δ (product_of_automata M₁ M₂).q₀ x =
+  ((List.foldl M₁.δ M₁.q₀ x), (List.foldl M₂.δ M₂.q₀ x)) := by
+  simp
+  exact
+  List.foldl_hom₂ x Prod.mk M₁.δ M₂.δ (fun x s ↦ (M₁.δ x.1 s, M₂.δ x.2 s)) M₁.q₀ M₂.q₀ fun a b ↦
+  congrFun rfl
+
+
+open Set
+-- have h : M = prod of automata
+theorem regular_languages_closed_under_union (M₁ : DFA Q₁ σ) (M₂ : DFA Q₂ σ)
+: ∃ Q : Type (max u w), ∃ (M : DFA Q σ), L M = L M₁ ∪ L M₂ := by
+exists Q₁ × Q₂
+exists product_of_automata M₁ M₂
+unfold L
+rw[Subset.antisymm_iff,subset_def,subset_def]
+simp only [acceptsFrom,evalFrom]
+constructor
+· intro x hx;
+  cases hx with
+  | inl hl =>
+    rw[foldl_prod_eq M₁ M₂ x] at hl; simp at hl
+    exact Or.inl hl
+  | inr hr =>
+    rw[foldl_prod_eq M₁ M₂ x] at hr; simp at hr
+    exact Or.inr hr
+· intro x hx
+  cases hx with
+  | inl hl =>
+  exact Or.inl (by rw[foldl_prod_eq M₁ M₂ x]; simp; exact hl)
+  | inr hr =>
+  exact Or.inr (by rw[foldl_prod_eq M₁ M₂ x]; simp; exact hr)
+
+
+end DFA
+
+structure NFA (Q : Type u) (σ : Type v) where
+  δ : Q → σ → Set Q
+  q₀ : Q
+  F : Set Q
+
+namespace NFA
+
+
+def stepSet (M : NFA Q σ) (S : Set Q) (a : σ) : Set Q :=
+  ⋃ s ∈ S, M.δ  s a
+
+theorem mem_stepSet {s : Q} {S : Set Q} {a : σ} (M : NFA Q σ) :
+s ∈ stepSet M S a ↔ ∃ t ∈ S, s ∈ M.δ t a := by
+  simp [stepSet]
+
+@[simp]
+theorem stepSet_empty (M : NFA Q σ) (a : σ) : stepSet M ∅ a = ∅ := by simp [stepSet]
+
+@[simp]
+theorem stepSet_singleton (M : NFA Q σ) (s : Q) (a : σ) : stepSet M {s} a = M.δ s a := by
+  simp [stepSet]
+
+
+/-- `M.evalFrom S x` computes all possible paths through `M` with input `x` starting at an element
+  of `S`. -/
+def evalFrom (M : NFA Q σ) (S : Set Q) : List σ → Set Q :=
+  List.foldl (stepSet M) S
+
+@[simp]
+theorem evalFrom_nil (M : NFA Q σ) (S : Set Q) : evalFrom M S [] = S :=
+  rfl
+
+@[simp]
+theorem evalFrom_singleton (M : NFA Q σ) (S : Set Q) (a : σ) :
+evalFrom M S [a] = stepSet M S a :=
+  rfl
+
+@[simp]
+theorem evalFrom_cons (M : NFA Q σ) (S : Set Q) (a : σ) (x : List σ) :
+    evalFrom M S (a :: x) = evalFrom M (stepSet M S a) x :=
+  rfl
+
+
+@[simp]
+theorem evalFrom_append_singleton (M : NFA Q σ) (S : Set Q) (x : List σ) (a : σ) :
+    evalFrom M S (x ++ [a]) = stepSet M (evalFrom M S x) a := by
+  simp only [evalFrom, List.foldl_append, List.foldl_cons, List.foldl_nil]
+
+
+variable (M) in
+@[simp]
+theorem evalFrom_biUnion (M : NFA Q σ) {ι : Type*} (t : Set ι) (f : ι → Set Q) :
+    ∀ (x : List σ), evalFrom M (⋃ i ∈ t, f i) x = ⋃ i ∈ t, evalFrom M (f i) x
+  | [] => by simp
+  | a :: x => by simp [stepSet, evalFrom_biUnion M _ _ x];
+
+
+theorem evalFrom_eq_biUnion_singleton (M : NFA Q σ) (S : Set Q) (x : List σ) :
+    evalFrom M S x = ⋃ s ∈ S, evalFrom M {s} x := by
+  simp [← evalFrom_biUnion]
+
+
+theorem mem_evalFrom_iff_exists (M : NFA Q σ) {s : Q} {S : Set Q} {x : List σ} :
+    s ∈ evalFrom M S x ↔ ∃ t ∈ S, s ∈ evalFrom M {t} x := by
+  rw [evalFrom_eq_biUnion_singleton]
+  simp
+
+
+/-- `M.eval x` computes all possible paths though `M` with input `x` starting at an element of
+  `M.start`. -/
+def eval (M : NFA Q σ) : List σ → Set Q :=
+  evalFrom M {M.q₀}
+
+
+@[simp]
+theorem eval_nil (M : NFA Q σ) : eval M [] = {M.q₀}  :=
+  rfl
+
+variable (M) in
+@[simp]
+theorem eval_singleton (M : NFA Q σ) (a : σ) : eval M [a] = stepSet M {M.q₀} a :=
+  rfl
+
+variable (M) in
+@[simp]
+theorem eval_append_singleton (M : NFA Q σ) (x : List σ) (a : σ) :
+eval M (x ++ [a]) = stepSet M (eval M x) a :=
+  evalFrom_append_singleton ..
+
+variable (M) in
+/-- `M.accepts` is the language of `x` such that there is an accept state in `M.eval x`. -/
+def L (M : NFA Q σ): Set (List σ) := {x | ∃ S ∈ M.F, S ∈ eval M x}
+
+theorem mem_accepts {x : List σ} (M : NFA Q σ) :
+x ∈ L M ↔ ∃ S ∈ M.F, S ∈ evalFrom M {M.q₀} x := by
+  rfl
+
+end NFA
